added compact printing in the SquiggleEq library.
used it to define compact (not necessarily pretty) printing for L4a.
(also updated SquiggleEq to the latest version fef0f1dfacc6b636a129558ee8e9836eb77476f1)
Although it produces decent results on simple examples, it
runs into stack overflow when printing Gcd (compiled to L4a).

Also, Quoting Gcd is very slow -- takes almost a minute.
In contrast, Extraction is very fast on Gcd.

certicoq/libraries/SquiggleEq/substitution.v
@@ -85,7 +85,8 @@ Generalizable Variable Opid.
 
 Section SubstGeneric.
 
-Context {NVar VarClass} {deqnvar : Deq NVar} {varclass: @VarType NVar VarClass deqnvar}
+Context {NVar VarClass} {deqnvar : Deq NVar} {varcl freshv} 
+{varclass: @VarType NVar VarClass deqnvar varcl freshv}
   `{hdeq: Deq Opid} {gts : GenericTermSig Opid}.
 Notation NTerm := (@NTerm NVar Opid).
 Notation BTerm := (@BTerm NVar Opid).
@@ -1062,20 +1063,25 @@ Fixpoint ssubst_aux {NVar} `{Deq NVar} {Opid} (nt : @NTerm NVar Opid) (sub : Sub
 *)
 
 
-Fixpoint change_bvars_alpha {NVar VarClass : Type} `{VarType NVar VarClass} 
+Fixpoint change_bvars_alpha {NVar VarCl : Type}
+`{Deq NVar}
+    {fv : FreshVars NVar VarCl}
+    {vc : VarClass NVar VarCl}
 {Opid} (lv : list NVar ) (t : (@NTerm NVar Opid)) 
 : (@NTerm NVar Opid) :=
 match t with
 | vterm v => vterm v
-| oterm o lbt => oterm o (map (@change_bvars_alphabt NVar _ _ _ _ lv) lbt)
+| oterm o lbt => oterm o (map (@change_bvars_alphabt NVar _  _ fv vc Opid lv) lbt)
 end
-with change_bvars_alphabt {NVar VarClass : Type} `{VarType NVar VarClass}  
+with change_bvars_alphabt {NVar VarCl : Type} 
+`{Deq NVar}    {fv: FreshVars NVar VarCl}
+    {vc : VarClass NVar VarCl}
   {Opid} lv 
 (bt: @BTerm NVar Opid) 
 : (@BTerm NVar Opid):=
 match bt with
 | bterm blv bnt => 
-    let bnt' := @change_bvars_alpha NVar _ _ _ _  lv bnt in
+    let bnt' := change_bvars_alpha lv bnt in
   (* All boundvars are produced by the [freshReplacements] function,
     which produces unique (no_repeats) variables.
     Also, these variables are disjoint from the bound variables of
@@ -1087,6 +1093,7 @@ match bt with
 end.
 
 
+
 (** % \noindent \\* %
   When we define alpha equality in the next section, we prove that
 [change_bvars_alpha] returns a term which is alpha equal to the input.
@@ -1095,7 +1102,7 @@ Finally, here is the function that safely perfoms
 
 *)
 (*
-Fixpoint makeBvarsUnique1 {NVar VarClass : Type} `{VarType NVar VarClass} 
+Fixpoint makeBvarsUnique1 {NVar VarClass : Type}
 {gts : GenericTermSig} (lv : list NVar ) (t : (@NTerm NVar gts)) 
 : (@NTerm NVar gts * list NVar) :=
 match t with
@@ -1118,7 +1125,9 @@ end.
 *)
 Class FreeVars (T V:Type) := freevars : T -> list V.
 
-Fixpoint ssubst {NVar VarClass} {d : Deq NVar} {vc : @VarType NVar VarClass d} 
+Fixpoint ssubst {NVar VarCl} {d : Deq NVar}
+    {fv : FreshVars NVar VarCl}
+    {vc : VarClass NVar VarCl}
 {Opid}
   (t : @NTerm NVar Opid) (sub : @Substitution NVar Opid) : @NTerm NVar Opid:=
 match t with
@@ -1127,9 +1136,11 @@ match t with
     | Some st => st
     | None => t
     end
-| oterm op bts => oterm op (map (fun t => @ssubst_bterm NVar VarClass d vc Opid t sub) bts)
+| oterm op bts => oterm op (map (fun t => @ssubst_bterm NVar VarCl d _ _ Opid t sub) bts)
 end
-with ssubst_bterm  {NVar VarClass}  {d : Deq NVar} {vc : @VarType NVar VarClass d}
+with ssubst_bterm  {NVar VarCl}  {d : Deq NVar}
+    {fv : FreshVars NVar VarCl}
+    {vc : VarClass NVar VarCl}
    {Opid}
   (bt : @BTerm NVar Opid) (sub : Substitution) : @BTerm  NVar Opid :=
   match bt with
@@ -1148,7 +1159,8 @@ with ssubst_bterm  {NVar VarClass}  {d : Deq NVar} {vc : @VarType NVar VarClass 
 
 Section SubstGeneric2.
 Typeclasses eauto :=10.
-Context {NVar VarClass} {deqnvar : Deq NVar} {varclass: @VarType NVar VarClass deqnvar} 
+Context {NVar VarClass} {deqnvar : Deq NVar} {varcl freshv} 
+{varclass: @VarType NVar VarClass deqnvar varcl freshv} 
  `{hdeq : Deq Opid} {gts : GenericTermSig Opid}.
 Notation NTerm := (@NTerm NVar Opid).
 Notation BTerm := (@BTerm NVar Opid).
@@ -1354,11 +1366,15 @@ Lemma ssubst_aux_trivial :
     (forall v u, LIn (v, u) sub -> isprogram u # ! LIn v (free_vars t))
     -> ssubst_aux t sub = t.
 Proof using.
+  clear varclass varcl freshv.
   intros.
   apply ssubst_aux_trivial_cl.
   unfold isprogram in *. 
   firstorder.
 Qed.
+
+
+
 
 Lemma prog_sub_flatmap_range : forall (sub : @Substitution Opid), prog_sub sub
     -> flat_map free_vars (range sub) =[].
@@ -1609,6 +1625,7 @@ Lemma ssubst_aux_trivial2 :
     -> isprogram t
     -> ssubst_aux t sub = t.
 Proof using.
+  clear varclass varcl freshv.
   intros. apply @ssubst_aux_trivial2_cl;  unfold isprogram in *;
   firstorder.
 Qed.
@@ -1628,7 +1645,7 @@ Lemma ssubst_trivial2 :
     (forall v u, LIn (v, u) sub -> isprogram u)
     -> isprogram t
     -> ssubst t sub = t.
-Proof using.
+Proof using varclass.
   intros. apply ssubst_trivial2_cl;  unfold isprogram in *;
   firstorder.
 Qed.
@@ -2696,7 +2713,7 @@ Lemma apply_bterm_append_program_id:
     (forall nt, LIn nt lnt -> isprogram nt) ->
     (forall nt, LIn nt lnta -> isprogram nt) ->
     (apply_bterm bt lnt = apply_bterm bt (lnt++lnta)).
-Proof using.
+Proof using varclass.
  intros ?  ? ? Hisp Hnt Hnta. destruct bt as [lv nt].
   unfold apply_bterm. simpl.
   assert(length lv <= length lnt \/ length lnt < length lv ) as Hdi by omega.
@@ -3101,6 +3118,7 @@ Proof using.
   change_to_ssubst_aux4.
 Qed.
 
+(*
 Lemma sub_mk_renames_disjoint :
   forall l1 l2,
     disjoint l1 l2
@@ -3125,7 +3143,7 @@ Proof using.
   apply IHl1 with (lva:=lva) in d0.
   allrw; boolvar; sp.
 Qed.
-
+*)
 
 
 Ltac dsub_find sn :=
@@ -4360,7 +4378,7 @@ Proof using.
 Qed.
 
 Lemma lmap_apply_var2: forall (lvi lvo : list NVar) v,
- (fun t=> @ssubst _ _ _ _ Opid t (var_ren lvi lvo)) (vterm v)
+ (fun t=> @ssubst _ _ _ _ _ Opid t (var_ren lvi lvo)) (vterm v)
   = vterm (lmap_apply deq_nvar (combine lvi lvo) v).
 Proof using.
  intros. simpl. unfold ssubst. simpl. rewrite sub_lmap_find.
@@ -4514,7 +4532,7 @@ Theorem freevars_ssubst_allvars9:
        -> free_vars (ssubst_aux t (var_ren lvi lvo)) 
           = lvmap_lapply (combine lvi lvo) (free_vars t).
 Proof using.
-  clear varclass VarClass.
+  clear varclass varcl freshv VarClass.
   nterm_ind1 t as [v | o lbt Hind] Case;
   introv Hnr Hdis.
   - Case "vterm".
@@ -4713,7 +4731,7 @@ Qed.
 
 Section TempTemp.
 
-Notation ssubst := (@ssubst NVar _ _ _ Opid).
+Notation ssubst := (@ssubst NVar _ _ _ _ Opid).
 
 Lemma ssubst_trivial4 :
   forall t sub, disjoint (dom_sub sub) (free_vars t) 
@@ -6265,7 +6283,7 @@ Lemma in_range_iff :
   forall (t : NTerm) (sub : Substitution),
     LIn t (range sub) <=> {v : NVar $ LIn (v, t) sub}.
 Proof using.
-  clear gts.
+  clear gts varclass varcl freshv deqnvar VarClass.
   induction sub; simpl; split; intro k; sp; allsimpl; subst; discover; sp; cpx;
      eauto.
   apply IHsub in H. sp. exists v; sp. firstorder.
@@ -6371,6 +6389,7 @@ Lemma prog_sub_snoc :
   forall s v t,
     prog_sub (snoc s (v,t)) <=> (prog_sub s # isprogram t).
 Proof using.
+  clear  varclass varcl freshv deqnvar VarClass.
   introv.
   unfold prog_sub, sub_range_sat; split; intro k.
 
@@ -6480,7 +6499,20 @@ Proof using.
   rewrite disjoint_flat_map_l in Hf.
   auto.
 Qed.
+
 End TempTemp.
+
+Lemma getopid_ssubst_aux_var_ren : forall (a : NTerm) sub,
+   allvars_sub sub
+  -> getOpid (ssubst_aux a sub) = getOpid a.
+Proof using varcl freshv.
+  intros nt sub H.
+  destruct nt; auto.
+   apply isvarc_ssubst_vterm with (v:=n) in H.
+    simpl in *. unfold isvarc in H. dsub_find sc; auto.
+    destruct scs; auto. contradiction.
+Qed.
+
 End SubstGeneric2.
 
 Lemma dom_sub_map_range {NVar} {gtsi} {gtso} : forall (f : @NTerm NVar gtsi -> @NTerm NVar gtso) sub,
